
### **Completing the Square Solutions - Set 1**

#### **Problem 1.**
>**Equation:** \(x^2 - 6x + 5 = 0\)

**Steps:**

1. **Rewrite** the equation: \(x^2 - 6x = -5\).
2. **Complete the square**:

\[
x^2 - 6x + \left(\frac{6}{2}\right)^2 = -5 + \left(\frac{6}{2}\right)^2
\]

\[
x^2 - 6x + 9 = 4
\]

\[
(x - 3)^2 = 4
\]

3. **Solve** for \(x\):

\[
x - 3 = \pm 2
\]

\[
x = 3 \pm 2
\]

\[
x = 5 \text{ or } x = 1
\]

#### **Problem 2.**
>**Equation:** \(x^2 + 8x + 15 = 0\)

**Steps:**

1. **Rewrite** the equation: \(x^2 + 8x = -15\).
2. **Complete the square**:

\[
x^2 + 8x + \left(\frac{8}{2}\right)^2 = -15 + \left(\frac{8}{2}\right)^2
\]

\[
x^2 + 8x + 16 = 1
\]

\[
(x + 4)^2 = 1
\]

3. **Solve** for \(x\):

\[
x + 4 = \pm 1
\]

\[
x = -4 \pm 1
\]

\[
x = -3 \text{ or } x = -5
\]

#### **Problem 3.**
>**Equation:** \(2x^2 - 4x - 6 = 0\)

**Steps:**
1. **Divide** by 2: \(x^2 - 2x - 3 = 0\).
2. **Rewrite** the equation: \(x^2 - 2x = 3\).
3. **Complete the square**:

\[
x^2 - 2x + \left(\frac{2}{2}\right)^2 = 3 + \left(\frac{2}{2}\right)^2
\]

\[
x^2 - 2x + 1 = 4
\]

\[
(x - 1)^2 = 4
\]

4. **Solve** for \(x\):

\[
x - 1 = \pm 2
\]

\[
x = 1 \pm 2
\]

\[
x = 3 \text{ or } x = -1
\]

#### **Problem 4.**
>**Equation:** \(3x^2 - 12x + 7 = 0\)

**Steps:**

1. **Rewrite** the equation: \(3x^2 - 12x = -7\).
2. **Divide** by 3: \(x^2 - 4x = -\frac{7}{3}\).
3. **Complete the square**:

\[
x^2 - 4x + \left(\frac{4}{2}\right)^2 = -\frac{7}{3} + \left(\frac{4}{2}\right)^2
\]

\[
x^2 - 4x + 4 = -\frac{7}{3} + \frac{16}{3}
\]

\[
(x - 2)^2 = \frac{9}{3}
\]

\[
(x - 2)^2 = 3
\]

4. **Solve** for \(x\):

\[
x - 2 = \pm \sqrt{3}
\]

\[
x = 2 \pm \sqrt{3}
\]

#### **Problem 5.**
>**Equation:** \(4x^2 + 20x + 25 = 0\)

**Steps:**

1. **Rewrite** the equation: \(4x^2 + 20x = -25\).
2. **Divide** by 4: \(x^2 + 5x = -\frac{25}{4}\).
3. **Complete the square**:
\[
x^2 + 5x + \left(\frac{5}{2}\right)^2 = -\frac{25}{4} + \left(\frac{5}{2}\right)^2
\]

\[
x^2 + 5x + \frac{25}{4} = 0
\]

\[
\left(x + \frac{5}{2}\right)^2 = 0
\]

4. **Solve** for \(x\):

\[
x + \frac{5}{2} = 0
\]

\[
x = -\frac{5}{2}
\]

#### **Problem 6.**
>**Equation:** \(x^2 + 6x - 7 = 0\)

**Steps:**
1. **Rewrite** the equation: \(x^2 + 6x = 7\).
2. **Complete the square**:
\[
x^2 + 6x + \left(\frac{6}{2}\right)^2 = 7 + \left(\frac{6}{2}\right)^2
\]

\[
x^2 + 6x + 9 = 16
\]

\[
(x + 3)^2 = 16
\]

3. **Solve** for \(x\):
\[
x + 3 = \pm 4
\]

\[
x = -3 \pm 4
\]

\[
x = 1 \text{ or } x = -7
\]

#### **Problem 7.**
>**Equation:** \(x^2 - 10x + 24 = 0\)

**Steps:**

1. **Rewrite** the equation: \(x^2 - 10x = -24\).
2. **Complete the square**:

\[
x^2 - 10x + \left(\frac{10}{2}\right)^2 = -24 + \left(\frac{10}{2}\right)^2
\]

\[
x^2 - 10x + 25 = 1
\]

\[
(x - 5)^2 = 1
\]

3. **Solve** for \(x\):

\[
x - 5 = \pm 1
\]

\[
x = 5 \pm 1
\]

\[
x = 6 \text{ or } x = 4
\]

#### **Problem 8.**
>**Equation:** \(5x^2 + 14x - 3 = 0\)

**Steps:**
1. **Rewrite** the equation: \(5x^2 + 14x = 3\).
2. **Divide** by 5: \(x^2 + \frac{14}{5}x = \frac{3}{5}\).
3. **Complete

 the square**:
\[
x^2 + \frac{14}{5}x + \left(\frac{7}{5}\right)^2 = \frac{3}{5} + \left(\frac{7}{5}\right)^2
\]

\[
x^2 + \frac{14}{5}x + \frac{49}{25} = \frac{15 + 49}{25}
\]

\[
\left(x + \frac{7}{5}\right)^2 = \frac{64}{25}
\]

4. **Solve** for \(x\):
\[
x + \frac{7}{5} = \pm \frac{8}{5}
\]

\[
x = -\frac{7}{5} \pm \frac{8}{5}
\]

\[
x = \frac{1}{5} \text{ or } x = -\frac{15}{5} = -3
\]

#### **Problem 9.**
>**Equation:** \(x^2 + 2x - 8 = 0\)

**Steps:**
1. **Rewrite** the equation: \(x^2 + 2x = 8\).
2. **Complete the square**:

\[
x^2 + 2x + \left(\frac{2}{2}\right)^2 = 8 + \left(\frac{2}{2}\right)^2
\]

\[
x^2 + 2x + 1 = 9
\]

\[
(x + 1)^2 = 9
\]

3. **Solve** for \(x\):

\[
x + 1 = \pm 3
\]
\
\[
x = -1 \pm 3
\]

\[
x = 2 \text{ or } x = -4
\]

#### **Problem 10.**
>**Equation:** \(6x^2 - 5x - 6 = 0\)

**Steps:**

1. **Rewrite** the equation: \(6x^2 - 5x = 6\).
2. **Divide** by 6: \(x^2 - \frac{5}{6}x = 1\).
3. **Complete the square**:
\[
x^2 - \frac{5}{6}x + \left(\frac{5}{12}\right)^2 = 1 + \left(\frac{5}{12}\right)^2
\]

\[
x^2 - \frac{5}{6}x + \frac{25}{144} = 1 + \frac{25}{144}
\]

\[
\left(x - \frac{5}{12}\right)^2 = \frac{169}{144}
\]

4. **Solve** for \(x\):

\[
x - \frac{5}{12} = \pm \frac{13}{12}
\]

\[
x = \frac{5}{12} \pm \frac{13}{12}
\]

\[
x = \frac{18}{12} = \frac{3}{2} \text{ or } x = -\frac{8}{12} = -\frac{2}{3}
\]

#### **Problem 11.**
>**Equation:** \(x^2 - 8x + 16 = 0\)

**Steps:**

1. **Rewrite** the equation: \(x^2 - 8x = -16\).
2. **Complete the square**:

\[
x^2 - 8x + \left(\frac{8}{2}\right)^2 = -16 + \left(\frac{8}{2}\right)^2
\]

\[
x^2 - 8x + 16 = 0
\]

\[
(x - 4)^2 = 0
\]

3. **Solve** for \(x\):

\[
x - 4 = 0
\]

\[
x = 4
\]

#### **Problem 12.**
>**Equation:** \(2x^2 + 4x - 3 = 0\)

**Steps:**

1. **Rewrite** the equation: \(2x^2 + 4x = 3\).
2. **Divide** by 2: \(x^2 + 2x = \frac{3}{2}\).
3. **Complete the square**:

\[
x^2 + 2x + \left(\frac{2}{2}\right)^2 = \frac{3}{2} + \left(\frac{2}{2}\right)^2
\]

\[
x^2 + 2x + 1 = \frac{5}{2}
\]

\[
(x + 1)^2 = \frac{5}{2}
\]

4. **Solve** for \(x\):

\[
x + 1 = \pm \sqrt{\frac{5}{2}}
\]

\[
x = -1 \pm \sqrt{\frac{5}{2}}
\]