# Factoring Quadratic Equations: Techniques

Factoring quadratics is a foundational method for solving quadratic equations. It involves rewriting a quadratic expression in the form \( ax^2 + bx + c \) as a product of two binomials, typically resulting in a form like \( (x - r)(x - ) = 0 \). By factoring, we can solve for the values of \( x \) that satisfy the equation. This method relies on recognizing patterns and using specific strategies to simplify the expression.

## **1. The Basic Quadratic Form:**

A standard quadratic equation has the form:
\[
ax^2 + bx + c = 0
\]
where \( a \), \( b \), and \( c \) are constants, and \( a \neq 0 \). The goal in factoring is to express this as:
\[
(ax + p)(bx + q) = 0
\]
where \( p \) and \( q \) are constants determined by the relationship between \( a \), \( b \), and \( c \).

---

## **2. Factoring Simple Quadratics (when \( a = 1 \)):**

For quadratics where the leading coefficient \( a = 1 \), the equation takes the form:

\[
x^2 + bx + c = 0
\]

**Steps:**

- **Identify two numbers** that multiply to \( c \) (the constant term) and add to \( b \) (the coefficient of the linear term).
   
    > Example: Factor \( x^2 + 7x + 12 \).
    >
    - We need two numbers that multiply to 12 and add to 7. 
    - The numbers are 3 and 4, so we rewrite the quadratic as:
    >
\[
(x + 3)(x + 4) = 0
\]

- **Set each factor equal to zero** and solve for \( x \):

\[
x + 3 = 0 \quad \text{or} \quad x + 4 = 0
\]

   So the solutions are \( x = -3 \) and \( x = -4 \).
