# Algebra - "Solve for x" Challenge

## Problem Statement

Solve for $x$ and $y$. You should have coordinate pairs ($x$, $y$) for each equation:

\[
    2x^{4/3} + 5x^{3/4} = 6x^{4/3} - 3x^{3/4}
\]

---

## Step-by-Step Solution

To solve the equation:

\[ 2x^{4/3} + 5x^{3/4} = 6x^{4/3} - 3x^{3/4} \]

we can follow these steps:

## <span style="color: orange; font-weight:bold; font-style: normal">Step 1</span>: Combine like terms

First, let's group the terms involving \(x^{4/3}\) on one side and \(x^{3/4}\) on the other side. We do this by subtracting \(6x^{4/3}\) and adding \(3x^{3/4}\) to both sides of the equation:

\[
2x^{4/3} + 5x^{3/4} - 6x^{4/3} + 3x^{3/4} = 0
\]

Combine like terms:

\[
(2x^{4/3} - 6x^{4/3}) + (5x^{3/4} + 3x^{3/4}) = 0
\]
\[
-4x^{4/3} + 8x^{3/4} = 0
\]

## <span style="color: orange; font-weight:bold; font-style: normal">Step 2</span>: Isolate one of the terms

To simplify, isolate one of the terms. Here, isolate \(x^{4/3}\) or \(x^{3/4}\). Let's isolate \(x^{4/3}\):

\[
-4x^{4/3} = -8x^{3/4}
\]

Divide both sides by -4:

\[
x^{4/3} = 2x^{3/4}
\]

## <span style="color: orange; font-weight:bold; font-style: normal">Step 3</span>: Solve for \(x\)

To solve for \(x\), we need to eliminate the exponents. We can do this by dividing both sides by \(x^{3/4}\) to get:

\[
\frac{x^{4/3}}{x^{3/4}} = 2
\]

Apply the **Quotient Rule for Exponents** which states \(\frac{a^m}{a^n} = a^{m-n}\):

\[
x^{4/3 - 3/4} = 2
\]

First, find a common denominator to subtract the exponents:

\[
4/3 - 3/4
\]

Convert to a common denominator (which is 12):

\[
\frac{16}{12} - \frac{9}{12} = \frac{7}{12}
\]

So:

\[
x^{7/12} = 2
\]

## <span style="color: orange; font-weight:bold; font-style: normal">Step 4</span>: Solve for \(x\)

Raise both sides to the power of the reciprocal of \(7/12\) to solve for \(x\):

\[
x = 2^{12/7}
\]

## <span style="color: orange; font-weight:bold; font-style: normal">Step 5</span>: Simplify if necessary

This is already in its simplest form. 

## <span style="color: green; font-weight:bold; font-style: normal">Solution</span>:

The solution to the equation is:

\[
x = 2^{12/7}
\]

## Summary of Properties Used:

1. **Combining Like Terms**: To simplify the equation by grouping similar terms.
2. **Isolating Variables**: To simplify the equation to a form where the variable can be solved.
3. **Quotient Rule for Exponents**: To combine terms with exponents and solve for \(x\).
4. **Exponentiation**: To solve for \(x\) by raising both sides to the power of the reciprocal.


