# Solution to Puzzle #1

## **Solution Steps:**

Let's call the original number 10x + y, where x is the tens digit and y is the ones digit.

1. From clue 2, we know:  
   \( x + y = 9 \)

2. From clue 3, the reversed number is 10y + x.  
   So, \( (10y + x) = (10x + y) + 27 \).  
   Simplifying this:  
   \( 10y + x = 10x + y + 27 \)  
   \( 9y - 9x = 27 \)  
   \( y - x = 3 \)

Now, solve the two equations:
- \( x + y = 9 \)
- \( y - x = 3 \)

Adding these equations:
- \( 2y = 12 \)
- \( y = 6 \)

Substitute \( y = 6 \) into \( x + y = 9 \):
- \( x + 6 = 9 \)
- \( x = 3 \)

So, the number is **36**!