# Factoring of Quadratics - Solutions to Set 1

Using the factoring method to solve for the following quadratics expression.

### Problem 1 

>Problem Statement: \(6x^2 - 11x - 35\)

**Steps:**

1. **Identify** \(a = 6\), \(b = -11\), and \(c = -35\).
2. **Find two numbers** that multiply to \(a \cdot c = 6 \cdot (-35) = -210\) and add to \(b = -11\). These numbers are \(-15\) and \(14\) because \(-15 \cdot 14 = -210\) and \(-15 + 14 = -11\).
3. **Rewrite** the middle term using these numbers:

\[
6x^2 - 15x + 14x - 35
\]

4. **Factor by grouping**:

\[
(6x^2 - 15x) + (14x - 35)
\]

\[
3x(2x - 5) + 7(2x - 5)
\]

5. **Factor out** the common binomial factor:

\[
(3x + 7)(2x - 5)
\]

### **Problem 2.**

>Problem Statement:  \(x^2 + 10x + 24\)

**Steps:**

1. **Identify** \(a = 1\), \(b = 10\), and \(c = 24\).
2. **Find two numbers** that multiply to \(a \cdot c = 24\) and add to \(b = 10\). These numbers are \(4\) and \(6\) because \(4 \cdot 6 = 24\) and \(4 + 6 = 10\).
3. **Rewrite** the middle term using these numbers:

\[
x^2 + 4x + 6x + 24
\]

4. **Factor by grouping**:
\[
(x^2 + 4x) + (6x + 24)
\]

\[
x(x + 4) + 6(x + 4)
\]
5. **Factor out** the common binomial factor:

\[
(x + 4)(x + 6)
\]

### **Problem 3.**

>Problem Statement: \(\frac{1}{2}x^2 - \frac{5}{2}x + 3\)

**Steps:**

1. **Identify** \(a = \frac{1}{2}\), \(b = -\frac{5}{2}\), and \(c = 3\).
2. **Multiply** \(a\) and \(c\):

\[
\frac{1}{2} \cdot 3 = \frac{3}{2}
\]

3. **Find two numbers** that multiply to \(\frac{3}{2}\) and add to \(-\frac{5}{2}\). These numbers are \(-1\) and \(-\frac{3}{2}\) because \(-1 \cdot -\frac{3}{2} = \frac{3}{2}\) and \(-1 - \frac{3}{2} = -\frac{5}{2}\).
4. **Rewrite** the middle term using these numbers:

\[
\frac{1}{2}x^2 - x - \frac{3}{2}x + 3
\]

5. **Factor by grouping**:

\[
\frac{1}{2}x(x - 2) - \frac{3}{2}(x - 2)
\]

6. **Factor out** the common binomial factor:

\[
\frac{1}{2}(x - 2)(x - 3)
\]

### **Problem 4.**

>Problem Statement: \(4x^2 - 25\)
**Steps:**

1. **Recognize** this as a difference of squares:

\[
4x^2 - 25 = (2x)^2 - 5^2
\]

2. **Apply** the difference of squares formula \(a^2 - b^2 = (a - b)(a + b)\):
\[
(2x - 5)(2x + 5)
\]

### **Problem 5.**

>Problem Statement: \(2x^2 + 7x - 15\)

**Steps:**

1. **Identify** \(a = 2\), \(b = 7\), and \(c = -15\).
2. **Find two numbers** that multiply to \(a \cdot c = 2 \cdot (-15) = -30\) and add to \(b = 7\). These numbers are \(10\) and \(-3\) because \(10 \cdot -3 = -30\) and \(10 - 3 = 7\).
3. **Rewrite** the middle term using these numbers:

\[
2x^2 + 10x - 3x - 15
\]

4. **Factor by grouping**:

\[
(2x^2 + 10x) + (-3x - 15)
\]

\[
2x(x + 5) - 3(x + 5)
\]

5. **Factor out** the common binomial factor:

\[
(2x - 3)(x + 5)
\]

### **Problem 6.**

>Problem Statement: \(3x^2 - 12x - 45\)

**Steps:**

1. **Factor out** the common factor of \(3\):
   \[
   3(x^2 - 4x - 15)
   \]
2. **Identify** \(a = 1\), \(b = -4\), and \(c = -15\).
3. **Find two numbers** that multiply to \(a \cdot c = -15\) and add to \(b = -4\). These numbers are \(-5\) and \(3\) because \(-5 \cdot 3 = -15\) and \(-5 + 3 = -4\).
4. **Rewrite** the middle term using these numbers:

\[
x^2 - 5x + 3x - 15
\]

5. **Factor by grouping**:

\[
(x^2 - 5x) + (3x - 15)
\]

\[
x(x - 5) + 3(x - 5)
\]

6. **Factor out** the common binomial factor:

\[
(x - 5)(x + 3)
\]

7. **Multiply by the common factor**:

\[
3(x - 5)(x + 3)
\]

### **Problem 7.**

>Problem Statement: \(5x^2 + 23x + 12\)

**Steps:**

1. **Identify** \(a = 5\), \(b = 23\), and \(c = 12\).
2. **Find two numbers** that multiply to \(a \cdot c = 5 \cdot 12 = 60\) and add to \(b = 23\). These numbers are \(15\) and \(4\) because \(15 \cdot 4 = 60\) and \(15 + 4 = 23\).
3. **Rewrite** the middle term using these numbers:

\[
5x^2 + 15x + 4x + 12
\]

4. **Factor by grouping**:

\[
(5x^2 + 15x) + (4x + 12)
\]

\[
5x(x + 3) + 4(x + 3)
\]

5. **Factor out** the common binomial factor:
\[
(5x + 4)(x + 3)
\]

### **Problem 8.**

>Problem Statement: \(-3x^2 + 8x + 16\)

**Steps:**

1. **Factor out** the common factor of \(-1\):
\[
-1(3x^2 - 8x - 16)
\]

2. **Identify** \(a = 3\), \(b = -8\), and \(c = -16\).
3. **Find two numbers** that multiply to \(a \cdot c = 3 \cdot (-16) = -48\) and add to \(b = -8\). These numbers are \(-12\) and \(4\) because \(-12 \cdot 4 = -48\) and \(-12 + 4 = -8\).
4. **Rewrite** the middle term using these numbers:

\[
-1(3x^2 - 12x + 4x - 16)
\]

5. **Factor by grouping**:
\[
-1[(3x^2 - 12x) + (4x - 16)]
\]

\[
-1[3x(x - 4) + 4(x - 4)]
\]

6. **Factor out** the common binomial factor:

\[
-1(x - 4)(3x + 4)
\]

### **Problem 9.**

>Problem Statement: \(x^2 - 10x + 25\)

**Steps:**

1. **Recognize** this as a perfect square trinomial:

\[
x^2 - 10x + 25 = (x - 5)^2
\]

### **Problem 10.**

>Problem Statement: \(x^2 - 6x + 8\)

**Steps:**
1. **Identify** \(a = 1\), \(b = -6\), and \(c = 8\).
2. **Find two numbers** that multiply to \(a \cdot c = 8\) and add to \(b = -6\). These numbers are \(-2\) and \(-4\) because \(-2 \cdot -4 = 8\) and \(-2 - 4 = -6\).
3. **Rewrite** the middle term using these numbers:

\[
x^2 - 2x - 4x + 8
\]

4. **Factor by grouping**:

\[
(x^2 - 2x) + (-4x + 8)
\]

\[
x(x - 2) - 4(x - 2)
\]

5. **Factor out** the common binomial factor:

\[
(x - 2)(x - 4)
\]

### **Problem 11.**

>Problem Statement: \(x^2 + 4x + 8\)

**Steps:**

1. **Identify** \(a = 1\), \(b = 4\), and \(c = 8\).
2. **Find two numbers** that multiply to \(a \cdot c = 8\) and add to \(b = 4\). This quadratic does not factor nicely over the reals. 
3. **Use the quadratic formula** to find roots:

\[
x = \frac{-4 \pm \sqrt{4^2 - 4 \cdot 1 \cdot 8}}{2 \cdot 1}
\]

\[
x = \frac{-4 \pm \sqrt{16 - 32}}{2}
\]

\[
x = \frac{-4 \pm \sqrt{-16}}{2}
\]

\[
x = \frac{-4 \pm 4i}{2}
\]

\[
x = -2 \pm 2i
\]

Thus, the factors are:

\[
(x - (-2 + 2i))(x - (-2 - 2i)) = (x + 2 - 2i)(x + 2 + 2i)
\]

### **Problem 12.**

>Problem Statement: \(6x^2 + 11x - 35\)

**Steps:**

1. **Identify** \(a = 6\), \(b = 11\), and \(c = -35\).
2. **Find two numbers** that multiply to \(a \cdot c = 6 \cdot (-35) = -210\) and add to \(b = 11\). These numbers are \(15\) and \(-14\) because \(15 \cdot -14 = -210\) and \(15 - 14 = 11\).
3. **Rewrite** the middle term using these numbers:

\[
6x^2 + 15x - 4x - 35
\]

4. **Factor by grouping**:

\[
(6x^2 + 15x) - (4x + 35)
\]

\[
3x(2x + 5) - 7(2x + 5)
\]

5. **Factor out** the common binomial factor:

\[
(3x - 7)(2x + 5)
\]

These steps guide you through the process of factoring each quadratic expression. If you have any questions or need further clarification, feel free to ask!